\newcommand{\authorinfo}{Julian Deinert, Frederik Wille, Carolin Konietzny}
\newcommand{\titleinfo}{ALA 09 (HA) zum 26.06.2014}

% PREAMBLE ===============================================================

\documentclass[a4paper,11pt,fleqn]{scrartcl}
\usepackage[german,ngerman]{babel}
\usepackage[utf8]{inputenc}
\usepackage[T1]{fontenc}
\usepackage{lmodern}
\usepackage{amssymb}
\usepackage{amsmath}
\usepackage{enumerate}
\usepackage{fancyhdr}
\usepackage{pgfplots}
\usepackage{multicol}
\usetikzlibrary{calc}
\usetikzlibrary{patterns}

\author{\authorinfo}
\title{\titleinfo}
\date{\today}

\newcommand{\bra}[1]{\left(#1\right)}
\newcommand{\limnn}[2]{\lim\limits_{n \rightarrow #1}\bra{#2}}
\newcommand{\limn}[1]{\lim\limits_{n \rightarrow \infty}\bra{#1}}
\newcommand{\limx}[1]{\lim\limits_{x \rightarrow \infty}\bra{#1}}
\newcommand{\limz}[1]{\lim\limits_{z \rightarrow \infty}\bra{#1}}
\newcommand{\rowi}[1]{\sum_{i=#1}^{\infty}}
\newcommand{\row}{\rowi{0}}
\newcommand{\step}[1]{\textbf{#1}}
\newcommand{\dX}[1]{\, \mathrm{d}#1}
\newcommand{\dx}[0]{\dX{x}}
\newcommand{\dt}[0]{\dX{t}}

\begin{document}
\maketitle
\begin{enumerate}
    
\item[\textbf{1.}]
	\begin{itemize}
	\item[(i)]
		\begin{align*}
			f(x,y)&=2x^2y^2-3xy+4x+2\\
			\frac{\delta f}{\delta x}(x,y)&=4xy^2-3y+4\\
			\frac{\delta f}{\delta y}(x,y)&=4x^2y-3x\\
			&=4x^2y+x\\
		\end{align*}
	\item[(ii)]
		\begin{align*}
			f(x,y)&=\cos(x^2y)*e^{xy}\\
			\frac{\delta f}{\delta x}(x,y)&=-sin(x^2y)*e^{xy}*2xy+\cos(x^2y)*e^{xy}\\
			\frac{\delta f}{\delta y}(x,y)&=-sin(x^2y)*e^{xy}*x^2+\cos(x^2y)*e^{xy}\\
		\end{align*}
	\item[(iii)]
		\begin{align*}
			f(x,y)&=\frac{\sin(x)+\cos(y)}{x^2+y^2}\\
			\frac{\delta f}{\delta x}(x,y)&=\frac{ \left( \cos \left( x \right)+cos\left(y\right)\right)*\left(x^2+y^2\right)-\left(\sin(x)+\cos(y)\right)*2x }{\left(x^2+y^2\right)^2}\\
			\frac{\delta f}{\delta y}(x,y)&=\frac{\left(\sin (x)-\sin (y)\right)*\left(x^2+y^2\right)-\left(\sin(x)+\cos(y)\right)*2y}{\left(x^2+y^2\right)^2}
		\end{align*}
	\item[(iv)]
		\begin{align*}
			f(x,y)&=\sqrt{1-x^2-y^2}\\
			&=\left(1-x^2-y^2\right)^\frac{1}{2}\\
			\frac{\delta f}{\delta x}(x,y)&=\frac{1}{2}*\left(1-x^2-y^2\right)^{-\frac{1}{2}}*2x\\
			\frac{\delta f}{\delta y}(x,y)&=\frac{1}{2}*\left(1-x^2-y^2\right)^{-\frac{1}{2}}*2y
		\end{align*}
	\end{itemize}

\item[\textbf{2.}]
	\begin{align*}
		f(x,y)&=x^2y^3+ye^{x^2y}\\
		\frac{\delta f}{\delta x}(x,y)&=2xy^3+y^2*e^{x^2y}*2x\\
		\frac{\delta f}{\delta y}(x,y)&=3x^2y^2+x^2ye^{x^2y}\\
		\frac{\delta^2 f}{\delta x^2}(x,y)&=2y^3+y^2*e^{x^2y}*4x^2\\
		\frac{\delta^2 f}{\delta y^2}(x,y)&=6x^2y+x^2y^2e^{x^2y}\\
		\frac{\delta^2 f}{\delta x \delta y}(x,y)&=\left( \frac{\delta f}{\delta x}(x,y) \right)'=6xy^2+2x*\left( 2y*e^{x^2y} + ye^{x^2y}*x^2 \right)\\
		&=6xy^2+4xye^{x^2y}+2x^3e^{x^2y}\\
		\frac{\delta^2 f}{\delta y \delta x}(x,y)&=\left( \frac{\delta f}{\delta y}(x,y) \right)'=6xy^2+y*\left( 4xe^{x^2y}+2x^3ye^{x^2y} \right)\\
		&=6xy^2+4xye^{x^2y}+2x^3e^{x^2y}
	\end{align*}

\item[\textbf{3.}]
    

\item[\textbf{4.}]

\end{enumerate}
\end{document}
